proof/theories/Optimizer/Optimize_DataMap.v
@@ -131,9 +131,9 @@ Lemma body_writes_orig : forall (f : field) (v M : data) (k : meta_key) (e : env
   body_writes (r_body (orig_map_rule f v M k)) e p
   = (e, if data_eqb (field_value f e p) v then set_meta p k M else p).
 Proof.
-  intros f v M k e p Hfx Hld. cbn [orig_map_rule r_body body_writes].
+  intros f v M k e p Hfx Hld. unfold body_writes; cbn [orig_map_rule r_body body_res_state body_step].
   rewrite (eval_mcmp_point f v e p Hld (field_fixed_len_loaded f (List.length v) e p Hfx Hld)).
-  destruct (data_eqb (field_value f e p) v); [cbn [body_writes vsrc_loadable eval_vsrc] | reflexivity].
+  destruct (data_eqb (field_value f e p) v); [unfold body_writes; cbn [body_res_state body_step vsrc_loadable eval_vsrc] | reflexivity].
   reflexivity.
 Qed.
 
@@ -152,11 +152,11 @@ Lemma body_writes_merged : forall (f : field) (setname mapname : string)
         else p).
 Proof.
   intros f setname mapname v1 v2 M1 M2 k e p Hset Hmap Hfx1 Hfx2 Hld.
-  cbn [mk_map_rule r_body body_writes].
+  unfold body_writes; cbn [mk_map_rule r_body body_res_state body_step].
   rewrite (mapn_head_mem f setname v1 v2 e p Hset Hfx1 Hfx2 Hld).
   destruct (data_eqb v1 (field_value f e p) || data_eqb v2 (field_value f e p));
     [| reflexivity].
-  cbn [body_writes vsrc_loadable fields_loadable forallb].
+  unfold body_writes; cbn [body_res_state body_step vsrc_loadable fields_loadable forallb].
   rewrite Hld, Bool.andb_true_r.
   cbn [eval_vsrc apply_transforms map List.concat].
   rewrite app_nil_r, Hmap. reflexivity.
@@ -215,12 +215,12 @@ Proof.
       by (unfold eval_matchcond, match_loadable; cbn [fields_loadable forallb];
           rewrite Hld; reflexivity).
     assert (Hmerged_p : body_writes (r_body (mk_map_rule f setname mapname k)) e p = (e, p))
-      by (cbn [mk_map_rule r_body body_writes]; rewrite Hmcc; reflexivity).
+      by (unfold body_writes; cbn [mk_map_rule r_body body_res_state body_step]; rewrite Hmcc; reflexivity).
     assert (Horig1 : body_writes (r_body (orig_map_rule f v1 M1 k)) e p = (e, p))
-      by (cbn [orig_map_rule r_body body_writes];
+      by (unfold body_writes; cbn [orig_map_rule r_body body_res_state body_step];
           unfold eval_matchcond, match_loadable; rewrite Hld; reflexivity).
     assert (Horig2 : body_writes (r_body (orig_map_rule f v2 M2 k)) e p = (e, p))
-      by (cbn [orig_map_rule r_body body_writes];
+      by (unfold body_writes; cbn [orig_map_rule r_body body_res_state body_step];
           unfold eval_matchcond, match_loadable; rewrite Hld; reflexivity).
     rewrite Hmerged_p, Horig1. cbv iota beta.
     rewrite (dsl_step_limit_free (orig_map_rule f v2 M2 k) e p) by reflexivity.
@@ -237,14 +237,29 @@ Lemma outcome_mk_map_none : forall f setname mapname k e p,
   outcome (mk_map_rule f setname mapname k) e p = None.
 Proof. reflexivity. Qed.
 
+Lemma step_orig_map_none : forall f v M k e p,
+  fst (rule_step (orig_map_rule f v M k) e p) = None.
+Proof.
+  intros. unfold rule_step. cbn [orig_map_rule r_body body_step].
+  destruct (eval_matchcond (MCmp f CEq v) e p); reflexivity.
+Qed.
+Lemma step_mk_map_none : forall f setname mapname k e p,
+  fst (rule_step (mk_map_rule f setname mapname k) e p) = None.
+Proof.
+  intros. unfold rule_step. cbn [mk_map_rule r_body body_step].
+  destruct (eval_matchcond (MConcatSet [f] false setname) e p);
+    [destruct (vsrc_loadable (VMap [f] [] mapname) p) |]; reflexivity.
+Qed.
+
 Lemma eval_rules_mut_continue : forall r rest e p,
-  outcome r e p = None ->
+  fst (rule_step r e p) = None ->
   eval_rules_mut (r :: rest) e p
   = (let '(e', p') := dsl_step r e p in eval_rules_mut rest e' p').
 Proof.
-  intros r rest e p Ho. cbn [eval_rules_mut dsl_rule_step]. rewrite Ho.
-  destruct (rule_loadable r e p && rule_applies r e p);
-    destruct (dsl_step r e p) as [e' p']; reflexivity.
+  intros r rest e p Ho. cbn [eval_rules_mut].
+  unfold dsl_step, dsl_rule_step.
+  destruct (rule_step r e p) as [v [e' p']]. cbn [fst] in Ho. subst v.
+  reflexivity.
 Qed.
 
 (** *** THE per-pass STATE correctness (non-vacuous): replacing the two originals by
@@ -262,11 +277,11 @@ Theorem eval_rules_mut_map_merge : forall (f : field) (v1 v2 M1 M2 : data)
   = eval_rules_mut (orig_map_rule f v1 M1 k :: orig_map_rule f v2 M2 k :: rest) e p.
 Proof.
   intros f v1 v2 M1 M2 setname mapname k rest e p Hpl Hset Hmap Hfx1 Hfx2 Hne.
-  rewrite (eval_rules_mut_continue _ rest e p (outcome_mk_map_none f setname mapname k e p)).
-  rewrite (eval_rules_mut_continue _ _ e p (outcome_orig_map_none f v1 M1 k e p)).
+  rewrite (eval_rules_mut_continue _ rest e p (step_mk_map_none f setname mapname k e p)).
+  rewrite (eval_rules_mut_continue _ _ e p (step_orig_map_none f v1 M1 k e p)).
   rewrite (dsl_step_map_merge f v1 v2 M1 M2 setname mapname k e p Hpl Hset Hmap Hfx1 Hfx2 Hne).
   destruct (dsl_step (orig_map_rule f v1 M1 k) e p) as [e1 p1].
-  rewrite (eval_rules_mut_continue _ rest e1 p1 (outcome_orig_map_none f v2 M2 k e1 p1)).
+  rewrite (eval_rules_mut_continue _ rest e1 p1 (step_orig_map_none f v2 M2 k e1 p1)).
   reflexivity.
 Qed.
 
@@ -343,7 +358,7 @@ Lemma dsl_step_bare_offkey : forall f v1 v2 M1 M2 mapname k e p,
 Proof.
   intros f v1 v2 M1 M2 mapname k e p Hmap Hld H1 H2.
   rewrite (dsl_step_limit_free (mk_map_rule_bare f mapname k) e p) by reflexivity.
-  unfold dsl_writes. cbn [mk_map_rule_bare r_body body_writes].
+  unfold dsl_writes. unfold body_writes; cbn [mk_map_rule_bare r_body body_res_state body_step].
   cbn [vsrc_loadable fields_loadable forallb]. rewrite Hld, Bool.andb_true_r.
   rewrite eval_vsrc_vmap_single, Hmap.
   rewrite (map_lookup_data_offkey _ v1 v2 M1 M2 H1 H2). reflexivity.
